# 洪輝霖微積分Practice Ch 1.2

###### tags: `微積分題目紀錄`



## Exercise 1

### Statement

$\displaystyle \lim_{t\rightarrow (-1)^{-}} (t^6-3t^5-2t+5)$



### Solution

$\displaystyle \lim_{t\rightarrow (-1)^{-}} (t^6-3t^5-2t+5) = (-1)^6-3(-1)^5-2(-1)+5 = 1+3+2+5=11$



### Answer

$\displaystyle \lim_{t\rightarrow (-1)^{-}} (t^6-3t^5-2t+5) = 11$



## Exercise 2

### Statement

$\displaystyle \lim_{t\rightarrow -2} |x^3-3x^2-2x+1|$



### Solution

$\displaystyle \lim_{t\rightarrow -2} |x^3-3x^2-2x+1| = |(-2)^3-3(-2)^2-2(-2)+1| = |-8-12+4+1| = |-15| = 15$



### Answer

$\displaystyle \lim_{t\rightarrow -2} |x^3-3x^2-2x+1| = 15$



## Exercise 3

### Statement

$\displaystyle \lim_{t\rightarrow 1}(t^{2010}+t+1)^3$



### Solution

$\displaystyle \lim_{t\rightarrow 1}(t^{2010}+t+1)^3 = (1^{2010}+1+1)^3 = 27$



### Answer

$\displaystyle \lim_{t\rightarrow 1}(t^{2010}+t+1)^3 = 27$



## Exercise 4

### Statement

$\displaystyle \lim_{t\rightarrow 3} \sqrt{2t^2+3t-2}$



### Solution

$\displaystyle \lim_{t\rightarrow 3} \sqrt{2t^2+3t-2} = \sqrt{2\times3^2+3\times 3 -2} = 5$



### Answer

$\displaystyle \lim_{t\rightarrow 3} \sqrt{2t^2+3t-2} = 5$



## Exercise 5

### Statement

$\displaystyle \lim_{t\rightarrow 2} \sqrt[3]{(3x^2+4)(x+2)}$



### Solution

$\displaystyle \lim_{t\rightarrow 2} \sqrt[3]{(3x^2+4)(x+2)} = \sqrt[3]{(3\times2^2+4)(4)} = \sqrt[3]{64} = 4$



### Answer

$\displaystyle \lim_{t\rightarrow 2} \sqrt[3]{(3x^2+4)(x+2)} = 4$



## Exercise 6

### Statement

$\displaystyle \lim_{x\rightarrow 1} \dfrac{3x+5}{x^2-2x+3}$



### Solution

$\displaystyle \lim_{x\rightarrow 1} \dfrac{3x+5}{x^2-2x+3} = \dfrac{3(1)+5}{1^2-2+3}=4$



### Answer

$\displaystyle \lim_{x\rightarrow 1} \dfrac{3x+5}{x^2-2x+3} = 4$



## Exercise 7

### Statement

$\displaystyle \lim_{x\rightarrow 2} \dfrac{x^2-x-2}{x-2}$



### Solution

$\displaystyle \lim_{x\rightarrow 2} \dfrac{x^2-x-2}{x-2} = \lim_{x\rightarrow 2} \dfrac{(x-2)(x+1)}{x-2} = \lim_{x\rightarrow 2} x+1 = 3$



### Answer

$\displaystyle \lim_{x\rightarrow 2} \dfrac{x^2-x-2}{x-2} = 3$



## Exercise 8

### Statement

$\displaystyle \lim_{x\rightarrow 1} \dfrac{x^2+2x-3}{x^2-1}$



### Solution

$\displaystyle \lim_{x\rightarrow 1} \dfrac{x^2+2x-3}{x^2-1} = \lim_{x\rightarrow 1} \dfrac{(x+3)(x-1)}{(x-1)(x+1)} = \lim_{x\rightarrow 1} \dfrac{x+3}{x+1} = \dfrac{4}{2} = 2$



### Answer

$\displaystyle \lim_{x\rightarrow 1} \dfrac{x^2+2x-3}{x^2-1} = 2$



## Exercise 9

### Statement

$\displaystyle \lim_{x\rightarrow -1} \dfrac{x^2-x-2}{x^2+4x+3}$ 



### Solution

$\displaystyle \lim_{x\rightarrow -1} \dfrac{x^2-x-2}{x^2+4x+3} = \lim_{x\rightarrow -1}\dfrac{(x-2)(x+1)}{(x+3)(x+1)} = \lim_{x\rightarrow -1}\dfrac{x-2}{x+3} = -\dfrac{3}{2}$



### Answer

$\displaystyle \lim_{x\rightarrow -1} \dfrac{x^2-x-2}{x^2+4x+3} = -\dfrac{3}{2}$



## Exercise 10

### Statement

$\displaystyle \lim_{x\rightarrow 3}\dfrac{1}{x-3}(\dfrac{1}{x}-\dfrac{1}{3})$



### Solution

$\displaystyle \lim_{x\rightarrow 3}\dfrac{1}{x-3}(\dfrac{1}{x}-\dfrac{1}{3}) = \displaystyle \lim_{x\rightarrow 3} \dfrac{1}{x-3}\dfrac{3-x}{3x} = \lim_{x\rightarrow 3}\dfrac{-1}{3x} = -\dfrac{1}{9}$



### Answer

$\displaystyle \lim_{x\rightarrow 3}\dfrac{1}{x-3}(\dfrac{1}{x}-\dfrac{1}{3}) = -\dfrac{1}{9}$



## Exercise 11

### Statement

$\displaystyle \lim_{x\rightarrow 0}(\dfrac{1}{x}-\dfrac{1}{x^2+x})$



### Solution

$\displaystyle \lim_{x\rightarrow 0}(\dfrac{1}{x}-\dfrac{1}{x^2+x}) = \lim_{x\rightarrow 0}\dfrac{x^2+x-x}{x(x^2+x)} = \lim_{x\rightarrow 0}\dfrac{x^2}{x^3+x^2} = \lim_{x\rightarrow0 }\dfrac{1}{x+1} = 1$



### Answer

$\displaystyle \lim_{x\rightarrow 0}(\dfrac{1}{x}-\dfrac{1}{x^2+x}) = 1$



## Exercise 12

### Statement

$\displaystyle \lim_{x\rightarrow 1}(\dfrac{1}{x-1}-\dfrac{2}{x^2-1})$



### Solution

$\displaystyle \lim_{x\rightarrow 1}(\dfrac{1}{x-1}-\dfrac{2}{x^2-1}) = \lim_{x\rightarrow 1} \dfrac{x+1-2}{x^2-1} = \lim_{x\rightarrow 1} \dfrac{x-1}{x^2-1} = \lim_{x\rightarrow 1}\dfrac{1}{x+1} = \dfrac{1}{2}$



### Answer

$\displaystyle \lim_{x\rightarrow 1}(\dfrac{1}{x-1}-\dfrac{2}{x^2-1}) = \dfrac{1}{2}$



## Exercise 13

### Statement

$\displaystyle \lim_{x\rightarrow 1} \dfrac{x^3-1}{x-1}$



### Solution

$\displaystyle \lim_{x\rightarrow 1} \dfrac{x^3-1}{x-1} = \lim_{x\rightarrow 1}({x^2+x+1}) = 3$ 



### Answer

$\displaystyle \lim_{x\rightarrow 1} \dfrac{x^3-1}{x-1} = 3$



## Exercise 14

### Statement

$\displaystyle \lim_{x\rightarrow -2} \dfrac{3-\sqrt{5-2x}}{2+x}$



### Solution

$\displaystyle \lim_{x\rightarrow -2} \dfrac{3-\sqrt{5-2x}}{2+x} = \lim_{x\rightarrow -2}\dfrac{3-\sqrt{5-2x}}{2+x} \dfrac{3+\sqrt{5-2x}}{3+\sqrt{5-2x}} = \lim_{x\rightarrow -2}\dfrac{9-5+2x}{(2+x)(3+\sqrt{5-2x})} =\lim_{x\rightarrow -2}\dfrac{2}{3+\sqrt{5-2x}} = \dfrac{2}{3+\sqrt{5+4}} = \dfrac{1}{3}$



### Answer

$\displaystyle \lim_{x\rightarrow -2} \dfrac{3-\sqrt{5-2x}}{2+x} = \dfrac{1}{3}$



## Exercise 15

### Statement

$\displaystyle \lim_{x\rightarrow 0} \dfrac{\sqrt{x+3}-\sqrt{3}}{x}$



### Solution

$\displaystyle \lim_{x\rightarrow 0} \dfrac{\sqrt{x+3}-\sqrt{3}}{x} = \lim_{x\rightarrow 0} \dfrac{\sqrt{x+3}-\sqrt{3}}{x} \dfrac{\sqrt{x+3}+\sqrt{3}}{\sqrt{x+3}+\sqrt{3}} = \lim_{x\rightarrow 0}\dfrac{x+3-3}{x(\sqrt{x+3}+\sqrt{3})} = \lim_{x\rightarrow 0}\dfrac{1}{(\sqrt{x+3}+\sqrt{3})} = \dfrac{\sqrt{3}}{6}$



### Answer

$\displaystyle \lim_{x\rightarrow 0} \dfrac{\sqrt{x+3}-\sqrt{3}}{x} = \dfrac{\sqrt{3}}{6}$



## Exercise 16

### Statement

$\displaystyle \lim_{x\rightarrow 2} \dfrac{x-2}{1-\sqrt{x^2-3}}$



### Solution

$\displaystyle \lim_{x\rightarrow 2} \dfrac{x-2}{1-\sqrt{x^2-3}} = \lim_{x\rightarrow 2} \dfrac{(x-2)(1+\sqrt{x^2-3})}{1-(x^2-3)} = \lim_{x\rightarrow 2} \dfrac{(x-2)(1+\sqrt{x^2-3})}{-x^2+4} = \lim_{x\rightarrow 2} -\dfrac{(x-2)(1+\sqrt{x^2-3})}{x^2-4}$

$\displaystyle  \lim_{x\rightarrow 2} -\dfrac{(x-2)(1+\sqrt{x^2-3})}{x^2-4} = \lim_{x\rightarrow 2} -\dfrac{(1+\sqrt{x^2-3})}{x+2} = -\dfrac{1}{2}$



### Answer

$\displaystyle \lim_{x\rightarrow 2} \dfrac{x-2}{1-\sqrt{x^2-3}} = -\dfrac{1}{2}$



## Exercise 17

### Statement

$\displaystyle \lim_{x\rightarrow 1} \dfrac{\sqrt{5-x}-2}{\sqrt{2-x}-1}$



### Solution

$\displaystyle \lim_{x\rightarrow 1} \dfrac{\sqrt{5-x}-2}{\sqrt{2-x}-1} = \lim_{x\rightarrow 1}\dfrac{\sqrt{5-x}-2}{\sqrt{2-x}-1}\dfrac{\sqrt{2-x}+1}{\sqrt{2-x}+1}\dfrac{\sqrt{5-x}+2}{\sqrt{5-x}+2} = \lim_{x\rightarrow 1} \dfrac{(5-x-4)(\sqrt{2-x}+1)}{(2-x-1)(\sqrt{5-x}+2)} = \lim_{x\rightarrow 1} \dfrac{\sqrt{2-x}+1}{\sqrt{5-x}+2} = \dfrac{1}{2}$



### Answer

$\displaystyle \lim_{x\rightarrow 1} \dfrac{\sqrt{5-x}-2}{\sqrt{2-x}-1} = \dfrac{1}{2}$



## Exercise 18

### Statement

$\displaystyle \lim_{x\rightarrow 0}(\dfrac{1}{x}-\dfrac{1}{x\sqrt{x+1}})$



### Solution

$\displaystyle \lim_{x\rightarrow 0}(\dfrac{1}{x}-\dfrac{1}{x\sqrt{x+1}}) = \lim_{x\rightarrow 0} \dfrac{x\sqrt{x+1}-x}{x^2\sqrt{x+1}} = \lim_{x\rightarrow 0} \dfrac{x(\sqrt{x+1}-1)}{x^2\sqrt{x+1}} = \lim_{x\rightarrow 0} \dfrac{\sqrt{x+1}-1}{x\sqrt{x+1}}$

$\displaystyle \lim_{x\rightarrow 0} \dfrac{\sqrt{x+1}-1}{x\sqrt{x+1}} = \lim_{x\rightarrow 0} \dfrac{\sqrt{x+1}-1}{x\sqrt{x+1}} \dfrac{\sqrt{x+1}+1}{\sqrt{x+1}+1} = \lim_{x\rightarrow 0} \dfrac{x+1-1}{x(\sqrt{x+1})(\sqrt{x+1}+1)} = \lim_{x\rightarrow 0} \dfrac{1}{(\sqrt{x+1})(\sqrt{x+1}+1)} = \dfrac{1}{2}$



### Answer

$\displaystyle \lim_{x\rightarrow 0}(\dfrac{1}{x}-\dfrac{1}{x\sqrt{x+1}}) = \dfrac{1}{2}$





## Exercise 19

### Statement

$\displaystyle \lim_{x\rightarrow 0} (\dfrac{1}{x\sqrt{1-x}} - \dfrac{1}{x})$



### Solution

$\displaystyle \lim_{x\rightarrow 0} (\dfrac{1}{x\sqrt{1-x}} - \dfrac{1}{x}) = \lim_{x\rightarrow 0} \dfrac{x-x\sqrt{1-x}}{x^2\sqrt{1-x}} = \lim_{x\rightarrow 0} \dfrac{1-\sqrt{1-x}}{x\sqrt{1-x}}$

$\displaystyle \lim_{x\rightarrow 0} \dfrac{1-\sqrt{1-x}}{x\sqrt{1-x}} = \lim_{x\rightarrow 0} \dfrac{1-\sqrt{1-x}}{x\sqrt{1-x}} \dfrac{1+\sqrt{1-x}}{1+\sqrt{1-x}} = \lim_{x\rightarrow 0} \dfrac{1-1+x}{x(\sqrt{1-x})(1+\sqrt{1-x})} = \lim_{x\rightarrow 0}\dfrac{1}{(\sqrt{1-x})(1+\sqrt{1-x})} = \dfrac{1}{2}$



### Answer

$\displaystyle \lim_{x\rightarrow 0} (\dfrac{1}{x\sqrt{1-x}} - \dfrac{1}{x}) = \dfrac{1}{2}$



## Exercise 20

### Statement

$\displaystyle \lim_{x\rightarrow (-3)^-} [2x+3]$



### Solution

考慮：$x \rightarrow (-3)^-$，因此$x < -3$

因此$2x < -6$，且$2x+3 < -3$

故$\displaystyle \lim_{x\rightarrow (-3)^-} [2x+3] = -4$



### Answer

$\displaystyle \lim_{x\rightarrow (-3)^-} [2x+3] = -4$



## Exercise 21

### Statement

$\displaystyle \lim_{x\rightarrow 3^+} \dfrac{3x-1}{[8-2x]}$



### Solution

考慮：$x \rightarrow 3^+$，因此$x > 3$

故$8-2x < 2$

因此$\displaystyle \lim_{x\rightarrow 3^+} \dfrac{3x-1}{[8-2x]} = \dfrac{8}{1} = 8$



### Answer

$\displaystyle \lim_{x\rightarrow 3^+} \dfrac{3x-1}{[8-2x]} = 8$



## Exercise 22

### Statement

$\displaystyle \lim_{x\rightarrow \infty} \dfrac{2x^2-3x+1}{x^2+2}$



### Solution

$\displaystyle \lim_{x\rightarrow \infty} \dfrac{2x^2-3x+1}{x^2+2} = \lim_{x\rightarrow \infty} \dfrac{\dfrac{2x^2}{x^2}-\dfrac{3x}{x^2}+\dfrac{1}{x^2}}{\dfrac{x^2}{x^2}+\dfrac{2}{x^2}} = \lim_{x\rightarrow \infty}\dfrac{2-\dfrac{3x}{x^2}+\dfrac{1}{x^2}}{1+\dfrac{2}{x^2}} = 2$



### Answer

$\displaystyle \lim_{x\rightarrow \infty} \dfrac{2x^2-3x+1}{x^2+2} = 2$





## Exercise 23

### Statement

$\displaystyle \lim_{x\rightarrow -\infty} \dfrac{x^2+100}{x^3-x-3}$



### Solution

$\displaystyle \lim_{x\rightarrow -\infty} \dfrac{x^2+100}{x^3-x-3} = \lim_{x\rightarrow -\infty} \dfrac{\dfrac{x^2}{x^3}+\dfrac{100}{x^3}}{\dfrac{x^3}{x^3}-\dfrac{x}{x^3}-\dfrac{3}{x^3}} = \dfrac{0+0}{1-0-0} = 0$



### Answer

$\displaystyle \lim_{x\rightarrow -\infty} \dfrac{x^2+100}{x^3-x-3} = 0$



## Exercise 24

### Statement

$\displaystyle \lim_{x\rightarrow \infty} \dfrac{x^3+x}{2-x^2}$



### Solution

$\displaystyle \lim_{x\rightarrow \infty} \dfrac{x^3+x}{2-x^2} = \lim_{x\rightarrow \infty} \dfrac{\dfrac{x^3}{x^2}+\dfrac{x}{x^2}}{\dfrac{2}{x^2}-\dfrac{x^2}{x^2}} = \lim_{x\rightarrow \infty} \dfrac{x+\dfrac{1}{x}}{\dfrac{2}{x^2}-1} = \lim_{x\rightarrow \infty}-x = -\infty$



### Answer

$\displaystyle \lim_{x\rightarrow \infty} \dfrac{x^3+x}{2-x^2} = -\infty$



## Exercise 25

### Statement

$\displaystyle \lim_{x\rightarrow \infty} \dfrac{\sqrt{4x^2+3}}{x-1}$



### Solution

$\displaystyle \lim_{x\rightarrow \infty} \dfrac{\sqrt{4x^2+3}}{x-1} = \lim_{x\rightarrow \infty} \dfrac{|2x|\sqrt{1+\dfrac{3}{4x^2}}}{x-1} = \lim_{x\rightarrow \infty} \dfrac{2x\sqrt{1+\dfrac{3}{4x^2}}}{x-1} = \lim_{x\rightarrow \infty} \dfrac{2\sqrt{1+\dfrac{3}{4x^2}}}{1-\dfrac{1}{x}} = \dfrac{2\sqrt{1+0}}{1-0} = 2$



### Answer

$\displaystyle \lim_{x\rightarrow \infty} \dfrac{\sqrt{4x^2+3}}{x-1}  = 2$



## Exercise 26

### Statement

$\displaystyle \lim_{x\rightarrow -\infty} \dfrac{1-2x}{\sqrt{x^2+4x-1}}$



### Solution

$\displaystyle \lim_{x\rightarrow -\infty} \dfrac{1-2x}{\sqrt{x^2+4x-1}} = \lim_{x\rightarrow -\infty} \dfrac{1-2x}{|x|\sqrt{\dfrac{x^2}{x^2}+\dfrac{4x}{x^2}-\dfrac{1}{x^2}}} = \lim_{x\rightarrow -\infty} \dfrac{1-2x}{-x\sqrt{\dfrac{x^2}{x^2}+\dfrac{4x}{x^2}-\dfrac{1}{x^2}}} = \lim_{x\rightarrow -\infty} \dfrac{\dfrac{1}{x}-\dfrac{2x}{x}}{-\sqrt{\dfrac{x^2}{x^2}+\dfrac{4x}{x^2}-\dfrac{1}{x^2}}} = \dfrac{0-2}{-\sqrt{1+0-0}} = 2$



### Answer

$\displaystyle \lim_{x\rightarrow -\infty} \dfrac{1-2x}{\sqrt{x^2+4x-1}} = 2$



## Exercise 27

### Statement

$\displaystyle \lim_{x\rightarrow \infty} (\sqrt{x^2+3x}-x)$



### Solution

$\displaystyle \lim_{x\rightarrow \infty} (\sqrt{x^2+3x}-x) = \lim_{x\rightarrow \infty} (\sqrt{x^2+3}-x)\dfrac{\sqrt{x^2+3}+x}{\sqrt{x^2+3}+x} = \lim_{x\rightarrow \infty} \dfrac{x^2+3x-x^2}{\sqrt{x^2+3}+x} = \lim_{x\rightarrow \infty} \dfrac{3x}{\sqrt{x^2+3}+x}$

$\displaystyle \lim_{x\rightarrow \infty} \dfrac{3x}{\sqrt{x^2+3}+x} = \lim_{x\rightarrow \infty} \dfrac{3x}{x\sqrt{1+\dfrac{3}{x^2}}+x} = \lim_{x\rightarrow \infty} \dfrac{3}{\sqrt{1+\dfrac{3}{x^2}}+1} = \dfrac{3}{1+1} = \dfrac{3}{2}$



### Answer

$\displaystyle \lim_{x\rightarrow \infty} (\sqrt{x^2+3x}-x) = \dfrac{3}{2}$



## Exercise 28

### Statement

$\displaystyle \lim_{x\rightarrow -\infty} (\sqrt{x^2+3x}+x)$



### Solution

$\displaystyle \lim_{x\rightarrow -\infty} (\sqrt{x^2+3x}+x) = \lim_{x\rightarrow -\infty} (\sqrt{x^2+3x}+x)\dfrac{\sqrt{x^2+3x}-x}{\sqrt{x^2+3x}-x} = \lim_{x\rightarrow -\infty} \dfrac{x^2+3x-x^2}{\sqrt{x^2+3x}-x} = \lim_{x\rightarrow -\infty} \dfrac{3x}{\sqrt{x^2+3x}-x}$

$\displaystyle \lim_{x\rightarrow -\infty} \dfrac{3x}{\sqrt{x^2+3x}-x} = \lim_{x\rightarrow -\infty} \dfrac{3x}{|x|\sqrt{\dfrac{x^2}{x^2}+\dfrac{3x}{x^2}}-x} = \lim_{x\rightarrow -\infty} \dfrac{3x}{-x\sqrt{\dfrac{x^2}{x^2}+\dfrac{3x}{x^2}}-x} = \lim_{x\rightarrow -\infty} \dfrac{3}{-\sqrt{1+\dfrac{3x}{x^2}}-1} = \dfrac{3}{-1-1} = -\dfrac{3}{2}$



### Answer

$\displaystyle \lim_{x\rightarrow -\infty} (\sqrt{x^2+3x}+x) = -\dfrac{3}{2}$



## Exercise 29

### Statement

$\displaystyle \lim_{x\rightarrow 1^+} \dfrac{3x-2}{1-x^2}$



### Solution

$\displaystyle \lim_{x\rightarrow 1^+} \dfrac{3x-2}{1-x^2} = \dfrac{1}{0}$

考慮$1^+ > 1$，因此$1-x^2 < 0$，$3x-2>0$，分子分母上下異號，故$\displaystyle \lim_{x\rightarrow 1^+} \dfrac{3x-2}{1-x^2} = -\infty$ 



### Answer

$\displaystyle \lim_{x\rightarrow 1^+} \dfrac{3x-2}{1-x^2} = -\infty$



## Exercise 30

### Statement

$\displaystyle \lim_{x\rightarrow (-2)^+} \dfrac{x^2-5}{x+2}$



### Solution

$\displaystyle \lim_{x\rightarrow (-2)^+} \dfrac{x^2-5}{x+2} = \dfrac{-1}{0}$

考慮$x\rightarrow (-2)^+$，因此$x > -2$，因此$x+2 > 0$，$x^2-5 < 0$

分子分母上下異號，故$\displaystyle \lim_{x\rightarrow (-2)^+} \dfrac{x^2-5}{x+2} = -\infty$



### Answer

$\displaystyle \lim_{x\rightarrow (-2)^+} \dfrac{x^2-5}{x+2} = -\infty$

